Lynx/Term/Induction.lean
@@ -8,6 +8,7 @@ namespace Lynx
 @[induction_eliminator] public protected theorem Term.induct {motive : Term → Prop} (t : Term)
     (integer : ∀ n, motive (.integer n))
     (atom : ∀ s, motive (.atom s))
+    (function : ∀ id arity, motive (.function id arity))
     (pid : ∀ pid, motive (.pid pid))
     (tuple : ∀ xs, (∀ x ∈ xs, motive x) → motive (.tuple xs))
     (map : ∀ entries, (∀ k v, (k, v) ∈ entries → motive k ∧ motive v) →
@@ -18,7 +19,7 @@ namespace Lynx
     (motive_3 := fun entries => ∀ k v, (k, v) ∈ entries → motive k ∧ motive v)
     (motive_4 := fun xs => ∀ x ∈ xs, motive x)
     (motive_5 := fun entry => motive entry.1 ∧ motive entry.2)
-    integer atom pid tuple map nil cons ?_ ?_ ?_ ?_ ?_ ?_ t
+    integer atom function pid tuple map nil cons ?_ ?_ ?_ ?_ ?_ ?_ t
   · intro xs ih x hx
     exact ih x (by simpa using hx)
   · simp
